examples/crypto/cryptobox/Box.DH.fst
@@ -33,15 +33,18 @@ assume val dh_gen_key: unit -> St (dh_share*dh_exponent)
 
 type keysize = aeadKeySize AES_128_GCM
 type aes_key = lbytes keysize (* = b:bytes{B.length b = keysize} *)
-assume val hash: dh_element -> aes_key
+assume val hash: dh_element -> Tot aes_key
 
 (*
   Setting up a global log for AE.keys indexed by the ids of the public and private key involved.
 *)
 private type range = fun (k_id:ae_id) -> k:PlainDH.key{PlainDH.ae_key_get_index k = k_id}
 private let inv (f:MM.map' (ae_id) range) = True
-private let ae_key_log_region = new_region root
-private let ae_key_log = MM.alloc #ae_key_log_region #ae_id #range #inv
+
+assume val ae_key_log_region: (r:MR.rid{ extends r root /\ is_eternal_region r /\ is_below r root})
+//private let ae_key_log_region = new_region root
+assume val ae_key_log: MM.t ae_key_log_region ae_id range inv
+//private let ae_key_log = MM.alloc #ae_key_log_region #ae_id #range #inv
 
 noeq abstract type dh_pkey = 
   | DH_pkey:  #pk_id:id -> rawpk:dh_share -> dh_pkey
@@ -82,24 +85,42 @@ let coerce_keypair #i dh_ex =
   pk,sk
 
 
+val prf_odhT: dh_skey -> dh_pkey -> Tot aes_key
+let prf_odhT dh_sk dh_pk =
+  let pk_id = dh_pk.pk_id in
+  let sk_id = dh_sk.sk_id in
+  let i = generate_ae_id pk_id sk_id in
+  let raw_k = dh_exponentiate dh_pk.rawpk dh_sk.rawsk in
+  let k = hash raw_k in
+  k
+  
+
 (**
    If we prf_odh is true, the output of this function is random, if both 
    share and exponent are honest.
 *)
-
-// Weird bug here. Can assert(False)??
 val prf_odh: sk:dh_skey -> pk:dh_pkey -> ST (PlainDH.key)
-  ( requires (fun h0 -> True))
-  ( ensures (fun h0 k h1 -> False))
-    let i = generate_ae_id sk.sk_id pk.pk_id in
+  ( requires (fun h0 ->
+    let i = generate_ae_id pk.pk_id sk.sk_id in
+    ae_fixed i
+    /\ (ae_honest i \/ ae_dishonest i)
+  ))
+  ( ensures (fun h0 k h1 ->
+    let i = generate_ae_id pk.pk_id sk.sk_id in
     (PlainDH.ae_key_get_index k = i)
-    /\ ( (ae_honest i /\ prf_odh)
-	  ==> ( MR.witnessed (MM.contains ae_key_log i k) 
-	      /\ modifies_none h0 h1
-	    )
-      )
-    /\ ( (ae_dishonest i \/ ~prf_odh)
-	  ==> modifies_none h0 h1
+    /\ (ae_honest i \/ ae_dishonest i)
+    /\ (
+        ( (ae_honest i /\ prf_odh)
+	    ==> (
+	       MR.witnessed (MM.contains ae_key_log i k) 
+	      )
+        )
+        \/ 
+	( (ae_dishonest i \/ ~prf_odh)
+	    ==> (modifies_none h0 h1
+	       /\ leak_key k = prf_odhT sk pk
+	      )
+        )
       )
   ))
 let prf_odh dh_sk dh_pk =
@@ -116,8 +137,9 @@ let prf_odh dh_sk dh_pk =
       let k' = PlainDH.keygen i in
       MM.extend ae_key_log i k';
       k')
-  else
+  else(
+    assert(ae_dishonest i \/ ~prf_odh);
     let raw_k = dh_exponentiate dh_pk.rawpk dh_sk.rawsk in
     let hashed_raw_k = hash raw_k in
     let k=PlainDH.coerce_key i hashed_raw_k in
-    k
+    k)
